P256: Partial work on add, sub, opp
Partial work towards #218

src/Arithmetic/MontgomeryReduction/WordByWord/Abstract/Dependent/Definition.v
@@ -22,10 +22,11 @@ Section WordByWordMontgomery.
     {R : positive}
     {R_numlimbs : nat}
     {scmul : forall {n}, Z -> T n -> T (S n)} (* uses double-output multiply *)
-    {add : forall {n}, T n -> T n -> T (S n)} (* joins carry *)
-    {add' : forall {n}, T (S n) -> T n -> T (S (S n))} (* joins carry *)
+    {addT : forall {n}, T n -> T n -> T (S n)} (* joins carry *)
+    {addT' : forall {n}, T (S n) -> T n -> T (S (S n))} (* joins carry *)
     {drop_high : T (S (S R_numlimbs)) -> T (S R_numlimbs)} (* drops the highest limb *)
     {conditional_sub : T (S R_numlimbs) -> T R_numlimbs} (* computes [arg - N] if [N <= arg], and drops high bit *)
+    {sub_then_maybe_add : T R_numlimbs -> T R_numlimbs -> T R_numlimbs} (* computes [a - b + if (a - b) <? 0 then N else 0] *)
     (N : T R_numlimbs).
 
   (* Recurse for a as many iterations as A has limbs, varying A := A, S := 0, r, bounds *)
@@ -36,10 +37,10 @@ Section WordByWordMontgomery.
             (S : T (S R_numlimbs)).
     (* Given A, B < R, we want to compute A * B / R mod N. R = bound 0 * ... * bound (n-1) *)
     Local Definition A_a := dlet p := divmod _ A in p. Local Definition A' := fst A_a. Local Definition a := snd A_a.
-    Local Definition S1 := add _ S (scmul _ a B).
+    Local Definition S1 := addT _ S (scmul _ a B).
     Local Definition s := snd (divmod _ S1).
     Local Definition q := fst (Z.mul_split r s k).
-    Local Definition S2 := add' _ S1 (scmul _ q N).
+    Local Definition S2 := addT' _ S1 (scmul _ q N).
     Local Definition S3 := fst (divmod _ S2).
     Local Definition S4 := drop_high S3.
   End Iteration.
@@ -67,6 +68,13 @@ Section WordByWordMontgomery.
     Definition redc : T R_numlimbs
       := conditional_sub pre_redc.
   End loop.
+
+  Definition add (A B : T R_numlimbs) : T R_numlimbs
+    := conditional_sub (addT _ A B).
+  Definition sub (A B : T R_numlimbs) : T R_numlimbs
+    := sub_then_maybe_add A B.
+  Definition opp (A : T R_numlimbs) : T R_numlimbs
+    := sub (zero _) A.
 End WordByWordMontgomery.
 
 Create HintDb word_by_word_montgomery.
